<?xml version="1.0"?>
<rdf:RDF xmlns="http://ontologies.sparna.fr/sparnatural-config-core#"
     xml:base="http://ontologies.sparna.fr/sparnatural-config-core"
     xmlns:owl="http://www.w3.org/2002/07/owl#"
     xmlns:rdf="http://www.w3.org/1999/02/22-rdf-syntax-ns#"
     xmlns:xml="http://www.w3.org/XML/1998/namespace"
     xmlns:xsd="http://www.w3.org/2001/XMLSchema#"
     xmlns:rdfs="http://www.w3.org/2000/01/rdf-schema#"
     xmlns:sparnatural-config-core="http://data.sparna.fr/ontologies/sparnatural-config-core#">
    <owl:Ontology rdf:about="http://data.sparna.fr/ontologies/sparnatural-config-core"/>
    


    <!-- 
    ///////////////////////////////////////////////////////////////////////////////////////
    //
    // Annotation properties
    //
    ///////////////////////////////////////////////////////////////////////////////////////
     -->

    


    <!-- http://data.sparna.fr/ontologies/sparnatural-config-core#beginDateProperty -->

    <owl:AnnotationProperty rdf:about="http://data.sparna.fr/ontologies/sparnatural-config-core#beginDateProperty">
        <rdfs:comment xml:lang="en">Use this annotation to relate a Sparnatural time property to another property that specifies how the start / beginning date is expressed on resources in the underlying graph.
That other property can itself be annotated with a sparqlString annotation in the case it corresponds to a property path.</rdfs:comment>
        <rdfs:label xml:lang="en">begin date property</rdfs:label>
    </owl:AnnotationProperty>
    


    <!-- http://data.sparna.fr/ontologies/sparnatural-config-core#defaultLabelProperty -->

    <owl:AnnotationProperty rdf:about="http://data.sparna.fr/ontologies/sparnatural-config-core#defaultLabelProperty">
        <rdfs:comment xml:lang="en">Use this annotation to relate a class in a Sparnatural configuration to a property that will be used as the default to fetch the labels of instances of this class. When a user selects this class as a column in the result set, if the class has this annotation set, everything behaves as if the user had selected also the corresponding property to be included.
The label property may have no domain specified if you don&apos;t want it to be proposed to the user.
The property must have a range specified to a single class.</rdfs:comment>
        <rdfs:label xml:lang="en">default label property</rdfs:label>
    </owl:AnnotationProperty>
    


    <!-- http://data.sparna.fr/ontologies/sparnatural-config-core#enableNegation -->

    <owl:AnnotationProperty rdf:about="http://data.sparna.fr/ontologies/sparnatural-config-core#enableNegation">
        <rdfs:comment xml:lang="en">Set this annotation to &quot;true&quot; on a property to indicate that this property can be applied a negation pattern (FILTER NOT EXISTS { ... })</rdfs:comment>
        <rdfs:label xml:lang="en">enable negation</rdfs:label>
        <rdfs:range rdf:resource="http://www.w3.org/2001/XMLSchema#boolean"/>
    </owl:AnnotationProperty>
    


    <!-- http://data.sparna.fr/ontologies/sparnatural-config-core#enableOptional -->

    <owl:AnnotationProperty rdf:about="http://data.sparna.fr/ontologies/sparnatural-config-core#enableOptional">
        <rdfs:comment xml:lang="en">Set this annotation to &quot;true&quot; on a property to indicate that this property can be applied an optional pattern (OPTIONAL { ... })</rdfs:comment>
        <rdfs:label xml:lang="en">enable optional</rdfs:label>
        <rdfs:range rdf:resource="http://www.w3.org/2001/XMLSchema#boolean"/>
    </owl:AnnotationProperty>
    


    <!-- http://data.sparna.fr/ontologies/sparnatural-config-core#endDateProperty -->

    <owl:AnnotationProperty rdf:about="http://data.sparna.fr/ontologies/sparnatural-config-core#endDateProperty">
        <rdfs:comment xml:lang="en">Use this annotation to relate a Sparnatural time property to another property that specifies how the end / stop date is expressed on resources in the underlying graph.
That other property can itself be annotated with a sparqlString annotation in the case it corresponds to a property path.</rdfs:comment>
        <rdfs:label xml:lang="en">end date property</rdfs:label>
    </owl:AnnotationProperty>
    


    <!-- http://data.sparna.fr/ontologies/sparnatural-config-core#exactDateProperty -->

    <owl:AnnotationProperty rdf:about="http://data.sparna.fr/ontologies/sparnatural-config-core#exactDateProperty">
        <rdfs:comment xml:lang="en">Use this annotation to relate a Sparnatural time property to another property that specifies how an exact date is expressed on resources in the underlying graph.
That other property can itself be annotated with a sparqlString annotation in the case it corresponds to a property path.

Time properties already annotated with a beginDateProperty or endDateProperty can also be annotated with this exactDateProperty in cases where the dates of the resources in the underlying graph can be expressed either as time periods or as exact dates.</rdfs:comment>
        <rdfs:label xml:lang="en">exact date property</rdfs:label>
    </owl:AnnotationProperty>
    


    <!-- http://data.sparna.fr/ontologies/sparnatural-config-core#faIcon -->

    <owl:AnnotationProperty rdf:about="http://data.sparna.fr/ontologies/sparnatural-config-core#faIcon">
        <rdfs:comment xml:lang="en">The code of an icon in FontAwesome to be associated to an entity, typically a class. Exemples of codes are &quot;fas fa-user&quot; or &quot;fas fa-file&quot;.
Search in FontAwesome at https://fontawesome.com/icons</rdfs:comment>
        <rdfs:label xml:lang="en">fontawesome icon code</rdfs:label>
        <rdfs:subPropertyOf rdf:resource="http://data.sparna.fr/ontologies/sparnatural-config-core#icon"/>
    </owl:AnnotationProperty>
    


    <!-- http://data.sparna.fr/ontologies/sparnatural-config-core#highlightedIcon -->

    <owl:AnnotationProperty rdf:about="http://data.sparna.fr/ontologies/sparnatural-config-core#highlightedIcon">
        <rdfs:comment xml:lang="en">An icon to be associated to an entity when it is highlighted. This is typically the same icon as the one indicated in the icon property, but with inversed colors.</rdfs:comment>
        <rdfs:label xml:lang="en">highlighted icon</rdfs:label>
        <rdfs:subPropertyOf rdf:resource="http://data.sparna.fr/ontologies/sparnatural-config-core#icon"/>
    </owl:AnnotationProperty>
    


    <!-- http://data.sparna.fr/ontologies/sparnatural-config-core#icon -->

    <owl:AnnotationProperty rdf:about="http://data.sparna.fr/ontologies/sparnatural-config-core#icon">
        <rdfs:comment xml:lang="en">An icon to be associated with an entity, typically a class. This can be the URL to an icon file or another mean to specify an icon, like a reference in an icon library.</rdfs:comment>
        <rdfs:label xml:lang="en">icon</rdfs:label>
    </owl:AnnotationProperty>
    


    <!-- http://data.sparna.fr/ontologies/sparnatural-config-core#isMultilingual -->

    <owl:AnnotationProperty rdf:about="http://data.sparna.fr/ontologies/sparnatural-config-core#isMultilingual">
        <rdfs:comment xml:lang="en">Set this annotation to &quot;true&quot; on a property to indicate that the values can be multigual and require a filter on the language</rdfs:comment>
        <rdfs:label xml:lang="en">is multilingual</rdfs:label>
        <rdfs:range rdf:resource="http://www.w3.org/2001/XMLSchema#boolean"/>
    </owl:AnnotationProperty>
    


    <!-- http://data.sparna.fr/ontologies/sparnatural-config-core#order -->

    <owl:AnnotationProperty rdf:about="http://data.sparna.fr/ontologies/sparnatural-config-core#order">
        <sparnatural-config-core:order xml:lang="en">An ordering information associated with this entity. This can be the display order of this entity within a list, or the display order of instances of the annotated class in list of instances, or predicates of the annotated property in a list of predicates, etc.</sparnatural-config-core:order>
        <rdfs:label xml:lang="en">order</rdfs:label>
    </owl:AnnotationProperty>
    


    <!-- http://data.sparna.fr/ontologies/sparnatural-config-core#sparqlString -->

    <owl:AnnotationProperty rdf:about="http://data.sparna.fr/ontologies/sparnatural-config-core#sparqlString">
        <rdfs:comment xml:lang="en">The equivalent SPARQL string that will be inserted in the final query instead of the annotated property or class.
When used to annotate a property, this annotation must contain a valid SPARQL property path (usually a single property), expanded without using any prefixes (i.e. full URIs in brackets).
When used to annotate a class, this annotation must contain a class URI, expanded without using any prefixes (i.e. full URIs in brackets), or a piece of SPARQL that can be inserted instead of the class URI, e.g;

&quot;&lt;http://www.w3.org/2004/02/skos/core#Concept&gt; ; &lt;http://www.w3.org/2004/02/skos/core#inScheme&gt; &lt;http://myScheme&gt; .&quot;</rdfs:comment>
        <rdfs:label xml:lang="en">sparql string</rdfs:label>
        <rdfs:range rdf:resource="http://www.w3.org/2001/XMLSchema#string"/>
    </owl:AnnotationProperty>
    


    <!-- http://data.sparna.fr/ontologies/sparnatural-config-core#tooltip -->

    <owl:AnnotationProperty rdf:about="http://data.sparna.fr/ontologies/sparnatural-config-core#tooltip">
        <rdfs:comment xml:lang="en">The content of the tooltip to be associated with a class or a property in the Sparnatural configuration.</rdfs:comment>
        <rdfs:label xml:lang="en">tooltip</rdfs:label>
    </owl:AnnotationProperty>
    


    <!-- 
    ///////////////////////////////////////////////////////////////////////////////////////
    //
    // Object Properties
    //
    ///////////////////////////////////////////////////////////////////////////////////////
     -->

    


    <!-- http://data.sparna.fr/ontologies/sparnatural-config-core#AutocompleteProperty -->

    <owl:ObjectProperty rdf:about="http://data.sparna.fr/ontologies/sparnatural-config-core#AutocompleteProperty">
        <rdfs:subPropertyOf rdf:resource="http://data.sparna.fr/ontologies/sparnatural-config-core#SelectResourceProperty"/>
        <rdfs:comment xml:lang="en">Use this super property to classify properties in Sparnatural configuration for which an autocomplete search field should be displayed to select a value.

The autocomplete suggestions can be configured using a datasource annotation, that will typically hold a reference to a SPARQL query to generate the autocomplete suggestions.</rdfs:comment>
        <rdfs:label xml:lang="en">autocomplete property</rdfs:label>
    </owl:ObjectProperty>
    


    <!-- http://data.sparna.fr/ontologies/sparnatural-config-core#BooleanProperty -->

    <owl:ObjectProperty rdf:about="http://data.sparna.fr/ontologies/sparnatural-config-core#BooleanProperty">
        <rdfs:subPropertyOf rdf:resource="http://data.sparna.fr/ontologies/sparnatural-config-core#SparnaturalProperty"/>
        <rdfs:comment xml:lang="en">Use this super property to classify properties in Sparnatural configuration for which a choice between &quot;true&quot; and &quot;false&quot; should be proposed.</rdfs:comment>
        <rdfs:label xml:lang="en">boolean property</rdfs:label>
    </owl:ObjectProperty>
    


    <!-- http://data.sparna.fr/ontologies/sparnatural-config-core#GraphDBSearchProperty -->

    <owl:ObjectProperty rdf:about="http://data.sparna.fr/ontologies/sparnatural-config-core#GraphDBSearchProperty">
        <rdfs:subPropertyOf rdf:resource="http://data.sparna.fr/ontologies/sparnatural-config-core#SearchProperty"/>
        <rdfs:comment xml:lang="en">Use this super property to classify properties in Sparnatural configuration for that will act like search properties but will generate GraphDB specific SPARQL criteria to search in a Lucene connector (i.e. using http://www.ontotext.com/connectors/lucene#query, etc.)</rdfs:comment>
        <rdfs:label xml:lang="en">search property in GraphDB</rdfs:label>
    </owl:ObjectProperty>
    


    <!-- http://data.sparna.fr/ontologies/sparnatural-config-core#ListProperty -->

    <owl:ObjectProperty rdf:about="http://data.sparna.fr/ontologies/sparnatural-config-core#ListProperty">
        <rdfs:subPropertyOf rdf:resource="http://data.sparna.fr/ontologies/sparnatural-config-core#SelectResourceProperty"/>
        <rdfs:comment xml:lang="en">Use this super property to classify properties in Sparnatural configuration for which a dropdown list should be displayed to select a value.

The list options can be configured using a datasource annotation, that will typically hold a reference to a SPARQL query to generate the list entries.</rdfs:comment>
        <rdfs:label xml:lang="en">list property</rdfs:label>
    </owl:ObjectProperty>
    


    <!-- http://data.sparna.fr/ontologies/sparnatural-config-core#LiteralListProperty -->

    <owl:ObjectProperty rdf:about="http://data.sparna.fr/ontologies/sparnatural-config-core#LiteralListProperty">
        <rdfs:subPropertyOf rdf:resource="http://data.sparna.fr/ontologies/sparnatural-config-core#SparnaturalProperty"/>
        <rdfs:comment xml:lang="en">Use this super property to classify properties in Sparnatural configuration for which a dropdown list should be displayed to select a _literal_ value. Use this when the list of distinct literal values is small (e.g. foaf:gender).

The list options can be configured using a datasource annotation, that will typically hold a reference to a SPARQL query to generate the list entries.</rdfs:comment>
        <rdfs:label xml:lang="en">literal list property</rdfs:label>
    </owl:ObjectProperty>
    


    <!-- http://data.sparna.fr/ontologies/sparnatural-config-core#NonSelectableProperty -->

    <owl:ObjectProperty rdf:about="http://data.sparna.fr/ontologies/sparnatural-config-core#NonSelectableProperty">
        <rdfs:subPropertyOf rdf:resource="http://data.sparna.fr/ontologies/sparnatural-config-core#SparnaturalProperty"/>
        <rdfs:comment xml:lang="en">Use this super property to classify properties in Sparnatural configuration for which no value selection widget (list, autocomplete field, etc.) should be displayed. Only a &quot;Where&quot; option is available to traverse the entity in the graph.

This is typically used to link entities that serve as connectors between other entities but that don&apos;t have intrinsic selection criterias by themselves, such as blank nodes or Activities in the CIDOC-CRM model.</rdfs:comment>
        <rdfs:label xml:lang="en">non-selectable property</rdfs:label>
    </owl:ObjectProperty>
    


    <!-- http://data.sparna.fr/ontologies/sparnatural-config-core#SearchProperty -->

    <owl:ObjectProperty rdf:about="http://data.sparna.fr/ontologies/sparnatural-config-core#SearchProperty">
        <rdfs:subPropertyOf rdf:resource="http://data.sparna.fr/ontologies/sparnatural-config-core#SparnaturalProperty"/>
        <rdfs:comment xml:lang="en">Use this super property to classify properties in Sparnatural configuration for which a simple text field should be used to enter a string to be searched for.</rdfs:comment>
        <rdfs:label xml:lang="en">search property</rdfs:label>
    </owl:ObjectProperty>
    


    <!-- http://data.sparna.fr/ontologies/sparnatural-config-core#SelectResourceProperty -->

    <owl:ObjectProperty rdf:about="http://data.sparna.fr/ontologies/sparnatural-config-core#SelectResourceProperty">
        <rdfs:subPropertyOf rdf:resource="http://data.sparna.fr/ontologies/sparnatural-config-core#SparnaturalProperty"/>
        <rdfs:comment xml:lang="en">The super-property of any property in a Sparnatural configuration for which a resource can be selected, through a list, an autocomplete field, or a tree.
Do not use this super-property directly, use its subproperties.</rdfs:comment>
        <rdfs:label xml:lang="en">select resource property</rdfs:label>
    </owl:ObjectProperty>
    


    <!-- http://data.sparna.fr/ontologies/sparnatural-config-core#SparnaturalProperty -->

    <owl:ObjectProperty rdf:about="http://data.sparna.fr/ontologies/sparnatural-config-core#SparnaturalProperty">
        <rdfs:comment xml:lang="en">Any property used to configure Sparnatural</rdfs:comment>
        <rdfs:label xml:lang="en">sparnatural property</rdfs:label>
    </owl:ObjectProperty>
    


    <!-- http://data.sparna.fr/ontologies/sparnatural-config-core#StringEqualsProperty -->

    <owl:ObjectProperty rdf:about="http://data.sparna.fr/ontologies/sparnatural-config-core#StringEqualsProperty">
        <rdfs:subPropertyOf rdf:resource="http://data.sparna.fr/ontologies/sparnatural-config-core#SearchProperty"/>
        <rdfs:comment xml:lang="en">Use this super property to classify properties in Sparnatural configuration for which a simple text field should be used to enter a string to be searched for, in an exact way, case-insensitive.</rdfs:comment>
        <rdfs:label xml:lang="en">string equals property</rdfs:label>
    </owl:ObjectProperty>
    


    <!-- http://data.sparna.fr/ontologies/sparnatural-config-core#TimeProperty -->

    <owl:ObjectProperty rdf:about="http://data.sparna.fr/ontologies/sparnatural-config-core#TimeProperty">
        <rdfs:subPropertyOf rdf:resource="http://data.sparna.fr/ontologies/sparnatural-config-core#SparnaturalProperty"/>
        <rdfs:comment xml:lang="en">The super-property of any property in a Sparnatural configuration for which a date range can be selected, using year or date picker.

Do not use this super-property directly, use its subproperties.</rdfs:comment>
        <rdfs:label xml:lang="en">time property</rdfs:label>
    </owl:ObjectProperty>
    


    <!-- http://data.sparna.fr/ontologies/sparnatural-config-core#TimeProperty-Date -->

    <owl:ObjectProperty rdf:about="http://data.sparna.fr/ontologies/sparnatural-config-core#TimeProperty-Date">
        <rdfs:subPropertyOf rdf:resource="http://data.sparna.fr/ontologies/sparnatural-config-core#TimeProperty"/>
        <rdfs:comment xml:lang="en">Use this super property to classify properties in Sparnatural configuration for which a datepicker with day/month/year precision should be displayed to select the beginning and end of a time span.</rdfs:comment>
        <rdfs:label xml:lang="en">time property with a date-picker</rdfs:label>
    </owl:ObjectProperty>
    


    <!-- http://data.sparna.fr/ontologies/sparnatural-config-core#TimeProperty-Period -->

    <owl:ObjectProperty rdf:about="http://data.sparna.fr/ontologies/sparnatural-config-core#TimeProperty-Period">
        <rdfs:subPropertyOf rdf:resource="http://data.sparna.fr/ontologies/sparnatural-config-core#TimeProperty"/>
        <rdfs:comment xml:lang="en">Use this super property to classify properties in Sparnatural configuration for which a datepicker with year precision combined with an autocomplete field on period name should be displayed to select the beginning and end of a time span.</rdfs:comment>
        <rdfs:label xml:lang="en">time property with chronocultural period selection</rdfs:label>
    </owl:ObjectProperty>
    


    <!-- http://data.sparna.fr/ontologies/sparnatural-config-core#TimeProperty-Year -->

    <owl:ObjectProperty rdf:about="http://data.sparna.fr/ontologies/sparnatural-config-core#TimeProperty-Year">
        <rdfs:subPropertyOf rdf:resource="http://data.sparna.fr/ontologies/sparnatural-config-core#TimeProperty"/>
        <rdfs:comment xml:lang="en">Use this super property to classify properties in Sparnatural configuration for which a datepicker with year precision should be displayed to select the beginning and end of a time span.</rdfs:comment>
        <rdfs:label xml:lang="en">time property with a year-picker</rdfs:label>
    </owl:ObjectProperty>
    


    <!-- http://data.sparna.fr/ontologies/sparnatural-config-core#TreeProperty -->

    <owl:ObjectProperty rdf:about="http://data.sparna.fr/ontologies/sparnatural-config-core#TreeProperty">
        <rdfs:subPropertyOf rdf:resource="http://data.sparna.fr/ontologies/sparnatural-config-core#SelectResourceProperty"/>
        <rdfs:comment xml:lang="en">Use this super property to classify properties in Sparnatural configuration for which a tree selection widget should be displayed.</rdfs:comment>
        <rdfs:label xml:lang="en">tree property</rdfs:label>
    </owl:ObjectProperty>
    


    <!-- 
    ///////////////////////////////////////////////////////////////////////////////////////
    //
    // Classes
    //
    ///////////////////////////////////////////////////////////////////////////////////////
     -->

    


    <!-- http://data.sparna.fr/ontologies/sparnatural-config-core#NotInstantiatedClass -->

    <owl:Class rdf:about="http://data.sparna.fr/ontologies/sparnatural-config-core#NotInstantiatedClass">
        <rdfs:subClassOf rdf:resource="http://data.sparna.fr/ontologies/sparnatural-config-core#SparnaturalClass"/>
        <rdfs:comment xml:lang="en">A &quot;Not-Instantiated-Class&quot; regroups all classes that are references to remote URIs, e.g. references to DBPedia URIs for indexing of LCSH languages, etc.
These URIs do not hold any information in the graph, but are useful to connect other entites.

  - a Not-Instantiated-Class cannot appear in initial list
  - a Not-Instantiated-Class must not yield an rdf:type criteria in the SPARQL query
  - a Not-Instantiated-Class can still be used to connect entites in the graph with a &quot;WHERE&quot; clause</rdfs:comment>
        <rdfs:label xml:lang="en">Not Instantiated Class</rdfs:label>
    </owl:Class>
    


    <!-- http://data.sparna.fr/ontologies/sparnatural-config-core#SparnaturalClass -->

    <owl:Class rdf:about="http://data.sparna.fr/ontologies/sparnatural-config-core#SparnaturalClass">
        <rdfs:comment xml:lang="en">Any class used to configure Sparnatural.</rdfs:comment>
        <rdfs:label xml:lang="en">Sparnatural class</rdfs:label>
    </owl:Class>
    


    <!-- http://www.w3.org/2000/01/rdf-schema#Literal -->

    <owl:Class rdf:about="http://www.w3.org/2000/01/rdf-schema#Literal">
        <rdfs:subClassOf rdf:resource="http://data.sparna.fr/ontologies/sparnatural-config-core#SparnaturalClass"/>
        <rdfs:comment xml:lang="en">The class rdfs:Literal is the class of literal values such as strings and integers. Property values such as textual strings are examples of RDF literals.

This is rdfs:Literal, provided here for being able to refer to it in Protege.

  - a Literal cannot appear in initial list
  - a Literal must not yield an rdf:type criteria in the SPARQL query
  - a Literal canot be used to connect entites in the graph with a &quot;WHERE&quot; clause
  - a Literal can only be used to place FILTER criterias on it</rdfs:comment>
        <rdfs:label xml:lang="en">Literal</rdfs:label>
    </owl:Class>
</rdf:RDF>



<!-- Generated by the OWL API (version 4.5.9.2019-02-01T07:24:44Z) https://github.com/owlcs/owlapi -->

